Source/Core/Parser.cs
@@ -595,10 +595,11 @@ private class BvBounds : Expr {
 		MoverType moverType = MoverType.None;
 		ActionDeclRef refinedAction = null;
 		List<Requires> pre = new List<Requires>();
+		List<Requires> preserves = new List<Requires>();
 		List<Ensures> post = new List<Ensures>();
 		List<CallCmd> yieldRequires = new List<CallCmd>();
-		List<CallCmd> yieldEnsures = new List<CallCmd>();
 		List<CallCmd> yieldPreserves = new List<CallCmd>();
+		List<CallCmd> yieldEnsures = new List<CallCmd>();
 		List<IdentifierExpr> mods = new List<IdentifierExpr>();
 		List<Variable> locals = null;
 		StmtList stmtList = null;
@@ -621,18 +622,18 @@ private class BvBounds : Expr {
 		if (la.kind == 10) {
 			Get();
 			while (StartOf(6)) {
-				SpecYieldPrePost(ref refinedAction, name, ins, outs, pre, post, yieldRequires, yieldEnsures, yieldPreserves, mods);
+				SpecYieldPrePost(ref refinedAction, name, ins, outs, pre, preserves, post, yieldRequires, yieldPreserves, yieldEnsures, mods);
 			}
 		} else if (StartOf(7)) {
 			while (StartOf(6)) {
-				SpecYieldPrePost(ref refinedAction, name, ins, outs, pre, post, yieldRequires, yieldEnsures, yieldPreserves, mods);
+				SpecYieldPrePost(ref refinedAction, name, ins, outs, pre, preserves, post, yieldRequires, yieldPreserves, yieldEnsures, mods);
 			}
 			ImplBody(out locals, out stmtList);
 			impl = new Implementation(name, name.val, new List<TypeVariable>(), Formal.StripWhereClauses(ins), Formal.StripWhereClauses(outs),
 			                         locals, stmtList, kv == null ? null : (QKeyValue)kv.Clone(), this.errors);
 			
 		} else SynErr(130);
-		ypDecl = new YieldProcedureDecl(name, name.val, moverType, ins, outs, pre, new List<Requires>(), mods, post, yieldRequires, yieldEnsures, yieldPreserves, refinedAction, kv); 
+		ypDecl = new YieldProcedureDecl(name, name.val, moverType, ins, outs, pre, preserves, post, mods, yieldRequires, yieldPreserves, yieldEnsures, refinedAction, kv); 
 	}
 
 	void Pure(ref bool isPure) {
@@ -670,7 +671,7 @@ private class BvBounds : Expr {
 			                         Formal.StripWhereClauses(ins), Formal.StripWhereClauses(outs), locals, stmtList, kv == null ? null : (QKeyValue)kv.Clone(), this.errors);
 			
 		} else SynErr(131);
-		proc = new Procedure(x, x.val, typeParams, ins, outs, isPure, pre, new List<Requires>(), mods, post, kv); 
+		proc = new Procedure(x, x.val, typeParams, ins, outs, isPure, pre, new List<Requires>(), post, mods, kv); 
 	}
 
 	void ActionDecl(bool isPure, out ActionDecl actionDecl, out Implementation impl, out DatatypeTypeCtorDecl datatypeTypeCtorDecl) {
@@ -748,7 +749,7 @@ private class BvBounds : Expr {
 		   datatypeTypeCtorDecl.AddConstructor(name, name.val, fields);
 		 }
 		}
-		actionDecl = new ActionDecl(name, name.val, moverType, ins, outs, isPure, creates, refinedAction, invariantAction, requires, yieldRequires, asserts, mods, datatypeTypeCtorDecl, kv);
+		actionDecl = new ActionDecl(name, name.val, moverType, ins, outs, isPure, creates, refinedAction, invariantAction, requires, mods, yieldRequires, asserts, datatypeTypeCtorDecl, kv);
 		
 	}
 
@@ -1236,7 +1237,7 @@ private class BvBounds : Expr {
 			 outParams.RemoveAll(x => x.HasAttribute(CivlAttributes.HIDE));
 			 var actionDecl = new ActionDecl(tok, actionName, moverType, Formal.StripWhereClauses(inParams), Formal.StripWhereClauses(outParams),
 			                               false, new List<ActionDeclRef>(), null, null,
-			                               new List<Requires>(), new List<CallCmd>(), new List<AssertCmd>(), new List<IdentifierExpr>(), null, akv);
+			                               new List<Requires>(), new List<IdentifierExpr>(), new List<CallCmd>(), new List<AssertCmd>(), null, akv);
 			 Pgm.AddTopLevelDeclaration(actionDecl);
 			 var impl = new Implementation(tok, actionDecl.Name, new List<TypeVariable>(), Formal.StripWhereClauses(inParams), Formal.StripWhereClauses(outParams),
 			                               locals, stmtList, akv == null ? null : (QKeyValue)akv.Clone());
@@ -1297,15 +1298,15 @@ private class BvBounds : Expr {
 		Expect(10);
 	}
 
-	void SpecYieldPrePost(ref ActionDeclRef refinedAction, IToken name, List<Variable> ins, List<Variable> outs, List<Requires> pre, List<Ensures> post, List<CallCmd> yieldRequires, List<CallCmd> yieldEnsures, List<CallCmd> yieldPreserves, List<IdentifierExpr> mods) {
+	void SpecYieldPrePost(ref ActionDeclRef refinedAction, IToken name, List<Variable> ins, List<Variable> outs, List<Requires> pre, List<Requires> preserves, List<Ensures> post, List<CallCmd> yieldRequires, List<CallCmd> yieldPreserves, List<CallCmd> yieldEnsures, List<IdentifierExpr> mods) {
 		if (la.kind == 42) {
 			SpecRefinedActionForYieldProcedure(ref refinedAction, name, ins, outs);
 		} else if (la.kind == 50) {
 			SpecYieldRequires(pre, yieldRequires);
+		} else if (la.kind == 37) {
+			SpecYieldPreserves(preserves, yieldPreserves);
 		} else if (la.kind == 51) {
 			SpecYieldEnsures(post, yieldEnsures);
-		} else if (la.kind == 37) {
-			SpecYieldPreserves(yieldPreserves);
 		} else if (la.kind == 54) {
 			SpecModifies(mods);
 		} else SynErr(141);
@@ -1346,6 +1347,23 @@ private class BvBounds : Expr {
 		
 	}
 
+	void SpecYieldPreserves(List<Requires> preserves, List<CallCmd> yieldPreserves ) {
+		Expr e; Cmd cmd; Token tok; QKeyValue kv = null; 
+		Expect(37);
+		tok = t; 
+		if (StartOf(17)) {
+			while (la.kind == 26) {
+				Attribute(ref kv);
+			}
+			Proposition(out e);
+			preserves.Add(new Requires(tok, false, e, null, kv)); 
+		} else if (la.kind == 39 || la.kind == 53 || la.kind == 71) {
+			CallCmd(true, out cmd);
+			yieldPreserves.Add((CallCmd)cmd); 
+		} else SynErr(142);
+		Expect(10);
+	}
+
 	void SpecYieldEnsures(List<Ensures> post, List<CallCmd> yieldEnsures ) {
 		Expr e; Cmd cmd; Token tok; QKeyValue kv = null; 
 		Expect(51);
@@ -1359,16 +1377,7 @@ private class BvBounds : Expr {
 		} else if (la.kind == 39 || la.kind == 53 || la.kind == 71) {
 			CallCmd(true, out cmd);
 			yieldEnsures.Add((CallCmd)cmd); 
-		} else SynErr(142);
-		Expect(10);
-	}
-
-	void SpecYieldPreserves(List<CallCmd> yieldPreserves ) {
-		Cmd cmd; Token tok; 
-		Expect(37);
-		tok = t; 
-		CallCmd(true, out cmd);
-		yieldPreserves.Add((CallCmd)cmd); 
+		} else SynErr(143);
 		Expect(10);
 	}
 
@@ -1399,7 +1408,7 @@ out List<Variable> ins, out List<Variable> outs, out QKeyValue kv) {
 			SpecPrePost(true, pre, post);
 		} else if (la.kind == 50 || la.kind == 51) {
 			SpecPrePost(false, pre, post);
-		} else SynErr(143);
+		} else SynErr(144);
 	}
 
 	void SpecPrePost(bool free, List<Requires> pre, List<Ensures> post) {
@@ -1422,7 +1431,7 @@ out List<Variable> ins, out List<Variable> outs, out QKeyValue kv) {
 			Proposition(out e);
 			Expect(10);
 			post.Add(new Ensures(tok, free, e, null, kv)); 
-		} else SynErr(144);
+		} else SynErr(145);
 	}
 
 	void StmtList(out StmtList stmtList) {
@@ -1516,7 +1525,7 @@ out List<Variable> ins, out List<Variable> outs, out QKeyValue kv) {
 				hideRevealId = new IdentifierExpr(t, t.val); 
 			} else if (la.kind == 60) {
 				Get();
-			} else SynErr(145);
+			} else SynErr(146);
 			c = hideRevealId == null ? new HideRevealCmd(t, mode) : new HideRevealCmd(hideRevealId, mode); 
 			Expect(10);
 		} else if (la.kind == 64) {
@@ -1563,7 +1572,7 @@ out List<Variable> ins, out List<Variable> outs, out QKeyValue kv) {
 			CallCmd(false, out cn);
 			Expect(10);
 			c = cn; 
-		} else SynErr(146);
+		} else SynErr(147);
 	}
 
 	void StructuredCmd(out StructuredCmd ec) {
@@ -1579,7 +1588,7 @@ out List<Variable> ins, out List<Variable> outs, out QKeyValue kv) {
 		} else if (la.kind == 61) {
 			BreakCmd(out bcmd);
 			ec = bcmd; 
-		} else SynErr(147);
+		} else SynErr(148);
 	}
 
 	void TransferCmd(out TransferCmd tc) {
@@ -1608,7 +1617,7 @@ out List<Variable> ins, out List<Variable> outs, out QKeyValue kv) {
 				Attribute(ref kv);
 			}
 			tc = new ReturnCmd(t) { Attributes = kv }; 
-		} else SynErr(148);
+		} else SynErr(149);
 		Expect(10);
 	}
 
@@ -1637,7 +1646,7 @@ out List<Variable> ins, out List<Variable> outs, out QKeyValue kv) {
 				Get();
 				StmtList(out els);
 				elseOption = els; 
-			} else SynErr(149);
+			} else SynErr(150);
 		}
 		ifcmd = new IfCmd(x, guard, thn, elseIfOption, elseOption, kv); 
 	}
@@ -1678,7 +1687,7 @@ out List<Variable> ins, out List<Variable> outs, out QKeyValue kv) {
 				yields.Add((CallCmd)cmd);
 				kv = null;
 				
-			} else SynErr(150);
+			} else SynErr(151);
 			Expect(10);
 		}
 		Expect(26);
@@ -1709,7 +1718,7 @@ out List<Variable> ins, out List<Variable> outs, out QKeyValue kv) {
 		} else if (StartOf(20)) {
 			Expression(out ee);
 			e = ee; 
-		} else SynErr(151);
+		} else SynErr(152);
 		Expect(12);
 	}
 
@@ -1787,7 +1796,7 @@ out List<Variable> ins, out List<Variable> outs, out QKeyValue kv) {
 			}
 			Expect(10);
 			c = new AssignCmd(x, lhss, rhss, kv); 
-		} else SynErr(152);
+		} else SynErr(153);
 	}
 
 	void MapAssignIndex(out IToken x, out List<Expr> indexes) {
@@ -1868,7 +1877,7 @@ out List<Variable> ins, out List<Variable> outs, out QKeyValue kv) {
 			}
 			Expect(12);
 			c = new CallCmd(x, first.val, es, ids, kv); ((CallCmd) c).IsFree = isFree; ((CallCmd) c).IsAsync = isAsync; 
-		} else SynErr(153);
+		} else SynErr(154);
 	}
 
 	void Expressions(out List<Expr> es) {
@@ -1913,7 +1922,7 @@ out List<Variable> ins, out List<Variable> outs, out QKeyValue kv) {
 			Get();
 		} else if (la.kind == 74) {
 			Get();
-		} else SynErr(154);
+		} else SynErr(155);
 	}
 
 	void LogicalExpression(out Expr e0) {
@@ -1951,7 +1960,7 @@ out List<Variable> ins, out List<Variable> outs, out QKeyValue kv) {
 			Get();
 		} else if (la.kind == 76) {
 			Get();
-		} else SynErr(155);
+		} else SynErr(156);
 	}
 
 	void ExpliesOp() {
@@ -1959,7 +1968,7 @@ out List<Variable> ins, out List<Variable> outs, out QKeyValue kv) {
 			Get();
 		} else if (la.kind == 78) {
 			Get();
-		} else SynErr(156);
+		} else SynErr(157);
 	}
 
 	void RelationalExpression(out Expr e0) {
@@ -1977,7 +1986,7 @@ out List<Variable> ins, out List<Variable> outs, out QKeyValue kv) {
 			Get();
 		} else if (la.kind == 80) {
 			Get();
-		} else SynErr(157);
+		} else SynErr(158);
 	}
 
 	void OrOp() {
@@ -1985,7 +1994,7 @@ out List<Variable> ins, out List<Variable> outs, out QKeyValue kv) {
 			Get();
 		} else if (la.kind == 82) {
 			Get();
-		} else SynErr(158);
+		} else SynErr(159);
 	}
 
 	void BvTerm(out Expr e0) {
@@ -2047,7 +2056,7 @@ out List<Variable> ins, out List<Variable> outs, out QKeyValue kv) {
 			x = t; op=BinaryOperator.Opcode.Ge; 
 			break;
 		}
-		default: SynErr(159); break;
+		default: SynErr(160); break;
 		}
 	}
 
@@ -2079,7 +2088,7 @@ out List<Variable> ins, out List<Variable> outs, out QKeyValue kv) {
 		} else if (la.kind == 92) {
 			Get();
 			x = t; op=BinaryOperator.Opcode.Sub; 
-		} else SynErr(160);
+		} else SynErr(161);
 	}
 
 	void Power(out Expr e0) {
@@ -2107,7 +2116,7 @@ out List<Variable> ins, out List<Variable> outs, out QKeyValue kv) {
 		} else if (la.kind == 95) {
 			Get();
 			x = t; op=BinaryOperator.Opcode.RealDiv; 
-		} else SynErr(161);
+		} else SynErr(162);
 	}
 
 	void IsConstructor(out Expr e0) {
@@ -2139,7 +2148,7 @@ out List<Variable> ins, out List<Variable> outs, out QKeyValue kv) {
 			e = Expr.Unary(x, UnaryOperator.Opcode.Not, e); 
 		} else if (StartOf(26)) {
 			CoercionExpression(out e);
-		} else SynErr(162);
+		} else SynErr(163);
 	}
 
 	void NegOp() {
@@ -2147,7 +2156,7 @@ out List<Variable> ins, out List<Variable> outs, out QKeyValue kv) {
 			Get();
 		} else if (la.kind == 99) {
 			Get();
-		} else SynErr(163);
+		} else SynErr(164);
 	}
 
 	void CoercionExpression(out Expr e) {
@@ -2171,7 +2180,7 @@ out List<Variable> ins, out List<Variable> outs, out QKeyValue kv) {
 				 e = new BvBounds(x, bn, ((LiteralExpr)e).asBigNum);
 				}
 				
-			} else SynErr(164);
+			} else SynErr(165);
 		}
 	}
 
@@ -2243,7 +2252,7 @@ out List<Variable> ins, out List<Variable> outs, out QKeyValue kv) {
 					Expression(out e1);
 					Expect(12);
 					e = new NAryExpr(x, new FieldUpdate(id, id.val), new List<Expr> { e, e1 }); 
-				} else SynErr(165);
+				} else SynErr(166);
 			}
 		}
 	}
@@ -2360,7 +2369,7 @@ out List<Variable> ins, out List<Variable> outs, out QKeyValue kv) {
 					e = new NAryExpr(x, new FunctionCall(id), es); 
 				} else if (la.kind == 12) {
 					e = new NAryExpr(x, new FunctionCall(id), new List<Expr>()); 
-				} else SynErr(166);
+				} else SynErr(167);
 				Expect(12);
 			}
 			break;
@@ -2420,7 +2429,7 @@ out List<Variable> ins, out List<Variable> outs, out QKeyValue kv) {
 				 e = new LambdaExpr(x, typeParams, ds, kv, e); 
 			} else if (la.kind == 9) {
 				LetExpr(out e);
-			} else SynErr(167);
+			} else SynErr(168);
 			Expect(12);
 			break;
 		}
@@ -2433,7 +2442,7 @@ out List<Variable> ins, out List<Variable> outs, out QKeyValue kv) {
 			e = new CodeExpr(locals, blocks); 
 			break;
 		}
-		default: SynErr(168); break;
+		default: SynErr(169); break;
 		}
 	}
 
@@ -2445,7 +2454,7 @@ out List<Variable> ins, out List<Variable> outs, out QKeyValue kv) {
 		} else if (la.kind == 6) {
 			Get();
 			s = t.val; 
-		} else SynErr(169);
+		} else SynErr(170);
 		try {
 		 n = BigDec.FromString(s);
 		} catch (FormatException) {
@@ -2487,7 +2496,7 @@ out List<Variable> ins, out List<Variable> outs, out QKeyValue kv) {
 			Get();
 		} else if (la.kind == 117) {
 			Get();
-		} else SynErr(170);
+		} else SynErr(171);
 	}
 
 	void QuantifierBody(IToken q, out List<TypeVariable> typeParams, out List<Variable> ds,
@@ -2505,7 +2514,7 @@ out QKeyValue kv, out Trigger trig, out Expr body) {
 			}
 		} else if (StartOf(12)) {
 			BoundVars(out ds);
-		} else SynErr(171);
+		} else SynErr(172);
 		QSep();
 		while (la.kind == 26) {
 			AttributeOrTrigger(ref kv, ref trig);
@@ -2518,7 +2527,7 @@ out QKeyValue kv, out Trigger trig, out Expr body) {
 			Get();
 		} else if (la.kind == 119) {
 			Get();
-		} else SynErr(172);
+		} else SynErr(173);
 	}
 
 	void Lambda() {
@@ -2526,7 +2535,7 @@ out QKeyValue kv, out Trigger trig, out Expr body) {
 			Get();
 		} else if (la.kind == 121) {
 			Get();
-		} else SynErr(173);
+		} else SynErr(174);
 	}
 
 	void LetExpr(out Expr letexpr) {
@@ -2641,7 +2650,7 @@ out QKeyValue kv, out Trigger trig, out Expr body) {
 			 Attributes = kv
 			}); 
 			
-		} else SynErr(174);
+		} else SynErr(175);
 		Expect(10);
 	}
 
@@ -2698,7 +2707,7 @@ out QKeyValue kv, out Trigger trig, out Expr body) {
 			 trig.AddLast(new Trigger(tok, true, es, null));
 			}
 			
-		} else SynErr(175);
+		} else SynErr(176);
 		Expect(27);
 	}
 
@@ -2713,7 +2722,7 @@ out QKeyValue kv, out Trigger trig, out Expr body) {
 		} else if (StartOf(20)) {
 			Expression(out e);
 			o = e; 
-		} else SynErr(176);
+		} else SynErr(177);
 	}
 
 	void QSep() {
@@ -2721,7 +2730,7 @@ out QKeyValue kv, out Trigger trig, out Expr body) {
 			Get();
 		} else if (la.kind == 123) {
 			Get();
-		} else SynErr(177);
+		} else SynErr(178);
 	}
 
 	void LetVar(out Variable v) {
@@ -2944,42 +2953,43 @@ public class Errors {
 			case 139: s = "invalid SpecRefinedActionForYieldProcedure"; break;
 			case 140: s = "invalid SpecYieldRequires"; break;
 			case 141: s = "invalid SpecYieldPrePost"; break;
-			case 142: s = "invalid SpecYieldEnsures"; break;
-			case 143: s = "invalid Spec"; break;
-			case 144: s = "invalid SpecPrePost"; break;
-			case 145: s = "invalid LabelOrCmd"; break;
+			case 142: s = "invalid SpecYieldPreserves"; break;
+			case 143: s = "invalid SpecYieldEnsures"; break;
+			case 144: s = "invalid Spec"; break;
+			case 145: s = "invalid SpecPrePost"; break;
 			case 146: s = "invalid LabelOrCmd"; break;
-			case 147: s = "invalid StructuredCmd"; break;
-			case 148: s = "invalid TransferCmd"; break;
-			case 149: s = "invalid IfCmd"; break;
-			case 150: s = "invalid WhileCmd"; break;
-			case 151: s = "invalid Guard"; break;
-			case 152: s = "invalid LabelOrAssign"; break;
-			case 153: s = "invalid CallParams"; break;
-			case 154: s = "invalid EquivOp"; break;
-			case 155: s = "invalid ImpliesOp"; break;
-			case 156: s = "invalid ExpliesOp"; break;
-			case 157: s = "invalid AndOp"; break;
-			case 158: s = "invalid OrOp"; break;
-			case 159: s = "invalid RelOp"; break;
-			case 160: s = "invalid AddOp"; break;
-			case 161: s = "invalid MulOp"; break;
-			case 162: s = "invalid UnaryExpression"; break;
-			case 163: s = "invalid NegOp"; break;
-			case 164: s = "invalid CoercionExpression"; break;
-			case 165: s = "invalid ArrayExpression"; break;
-			case 166: s = "invalid AtomExpression"; break;
+			case 147: s = "invalid LabelOrCmd"; break;
+			case 148: s = "invalid StructuredCmd"; break;
+			case 149: s = "invalid TransferCmd"; break;
+			case 150: s = "invalid IfCmd"; break;
+			case 151: s = "invalid WhileCmd"; break;
+			case 152: s = "invalid Guard"; break;
+			case 153: s = "invalid LabelOrAssign"; break;
+			case 154: s = "invalid CallParams"; break;
+			case 155: s = "invalid EquivOp"; break;
+			case 156: s = "invalid ImpliesOp"; break;
+			case 157: s = "invalid ExpliesOp"; break;
+			case 158: s = "invalid AndOp"; break;
+			case 159: s = "invalid OrOp"; break;
+			case 160: s = "invalid RelOp"; break;
+			case 161: s = "invalid AddOp"; break;
+			case 162: s = "invalid MulOp"; break;
+			case 163: s = "invalid UnaryExpression"; break;
+			case 164: s = "invalid NegOp"; break;
+			case 165: s = "invalid CoercionExpression"; break;
+			case 166: s = "invalid ArrayExpression"; break;
 			case 167: s = "invalid AtomExpression"; break;
 			case 168: s = "invalid AtomExpression"; break;
-			case 169: s = "invalid Dec"; break;
-			case 170: s = "invalid Forall"; break;
-			case 171: s = "invalid QuantifierBody"; break;
-			case 172: s = "invalid Exists"; break;
-			case 173: s = "invalid Lambda"; break;
-			case 174: s = "invalid SpecBlock"; break;
-			case 175: s = "invalid AttributeOrTrigger"; break;
-			case 176: s = "invalid AttributeParameter"; break;
-			case 177: s = "invalid QSep"; break;
+			case 169: s = "invalid AtomExpression"; break;
+			case 170: s = "invalid Dec"; break;
+			case 171: s = "invalid Forall"; break;
+			case 172: s = "invalid QuantifierBody"; break;
+			case 173: s = "invalid Exists"; break;
+			case 174: s = "invalid Lambda"; break;
+			case 175: s = "invalid SpecBlock"; break;
+			case 176: s = "invalid AttributeOrTrigger"; break;
+			case 177: s = "invalid AttributeParameter"; break;
+			case 178: s = "invalid QSep"; break;
 
 			default: s = "error " + n; break;
 		}
