Test/civl/samples/2pc.bpl
@@ -100,10 +100,8 @@ yield right procedure {:layer 1} vote_all(xid: TransactionId, {:linear_in} vrs: 
 requires {:layer 1} vrs == Set((lambda vr:VoteRequest :: vr->xid == xid && 1 <= vr->rid && vr->rid < i+1));
 ensures {:layer 1} (forall j:int :: 1 <= j && j < i+1 && votes[j] == YES() ==> Set_Contains(locked_transactions[j], xid));
 ensures {:layer 1} vrs' ==Set((lambda vr:VoteRequest :: vr->xid == xid && 1 <= vr->rid && vr->rid < i+1));
-requires {:layer 1} (forall  {:pool "J"} j:int, xid1: TransactionId, xid2: TransactionId :: {:add_to_pool "J", j} (1 <= j && j < n+1 && xid1 != xid2 && Set_Contains(locked_transactions[j], xid1) && Set_Contains(locked_transactions[j], xid2)) ==> !Conflict[xid1][xid2]);
-ensures {:layer 1} (forall  {:pool "J"} j:int, xid1: TransactionId, xid2: TransactionId :: {:add_to_pool "J", j} (1 <= j && j < n+1 && xid1 != xid2 && Set_Contains(locked_transactions[j], xid1) && Set_Contains(locked_transactions[j], xid2)) ==> !Conflict[xid1][xid2]);
-requires {:layer 1} (forall {:pool "J"} j:int, xid0: TransactionId :: {:add_to_pool "J", j} 1 <= j && j < n+1 && Set_Contains(committed_transactions, xid0) ==> Set_Contains(locked_transactions[j], xid0));
-ensures {:layer 1} (forall {:pool "J"} j:int, xid0: TransactionId :: {:add_to_pool "J", j} 1 <= j && j < n+1 && Set_Contains(committed_transactions, xid0) ==> Set_Contains(locked_transactions[j], xid0));
+preserves {:layer 1} LockedNoConflicts(locked_transactions);
+preserves {:layer 1} CommittedSubsetLocked(locked_transactions, committed_transactions);
 ensures {:layer 1} (forall j:int :: 1 <= j && j < n+1 ==> IsSubset(old(locked_transactions)[j]->val, locked_transactions[j]->val));
 ensures {:layer 1} (forall j:int :: 1 <= j && j < i+1 ==> votes[j] != NONE());
 modifies locked_transactions;
@@ -125,10 +123,8 @@ yield left procedure {:layer 1} finalize_all(d: Decision, {:linear} xid: One Tra
 requires {:layer 1} vrs == allVoteRequests(xid->val);
 requires {:layer 1}  (forall j:int :: {:add_to_pool "J", j} d == COMMIT() &&  1 <= j && j < n+1 ==> Set_Contains(locked_transactions[j], xid->val));
 ensures {:layer 1}  (forall j:int :: d == COMMIT() && 1 <=j && j < n+1 ==> Set_Contains(locked_transactions[j], xid->val));
-requires {:layer 1} (forall  {:pool "J"} j:int, xid1: TransactionId, xid2: TransactionId :: {:add_to_pool "J", j} (1 <= j && j < n+1 && xid1 != xid2 && Set_Contains(locked_transactions[j], xid1) && Set_Contains(locked_transactions[j], xid2)) ==> !Conflict[xid1][xid2]);
-ensures {:layer 1} (forall  {:pool "J"} j:int, xid1: TransactionId, xid2: TransactionId :: {:add_to_pool "J", j} (1 <= j && j < n+1 && xid1 != xid2 && Set_Contains(locked_transactions[j], xid1) && Set_Contains(locked_transactions[j], xid2)) ==> !Conflict[xid1][xid2]);
-requires {:layer 1} (forall {:pool "J"} j:int, xid0: TransactionId :: {:add_to_pool "J", j} 1 <= j && j < n+1 && Set_Contains(committed_transactions, xid0) ==> Set_Contains(locked_transactions[j], xid0));
-ensures {:layer 1} (forall {:pool "J"} j:int, xid0: TransactionId :: {:add_to_pool "J", j} 1 <= j && j < n+1 && Set_Contains(committed_transactions, xid0) ==> Set_Contains(locked_transactions[j], xid0));
+preserves {:layer 1} LockedNoConflicts(locked_transactions);
+preserves {:layer 1} CommittedSubsetLocked(locked_transactions, committed_transactions);
 requires {:layer 1} !Set_Contains(committed_transactions, xid->val);
 ensures {:layer 1} (forall j:int, xid0 : TransactionId :: 1 <= j && j < n+1 && xid0 != xid->val && Set_Contains(old(locked_transactions)[j], xid0) ==> Set_Contains(locked_transactions[j], xid0));
 modifies locked_transactions;
@@ -189,11 +185,23 @@ refines atomic action {:layer 1, 1} _ {
     committed_transactions := Set_Add(committed_transactions, xid->val);
 }
 
+function {:inline} LockedNoConflicts(locked_transactions: [ReplicaId](Set TransactionId)) : bool
+{
+    (forall  {:pool "J"} j: int, xid1: TransactionId, xid2: TransactionId :: {:add_to_pool "J", j}
+        1 <= j && j < n+1 && xid1 != xid2 && Set_Contains(locked_transactions[j], xid1) && Set_Contains(locked_transactions[j], xid2)
+        ==> !Conflict[xid1][xid2])
+}
 yield invariant {:layer 1} LockedNoConflicts();
-preserves {:layer 1} (forall  {:pool "J"} j:int, xid1: TransactionId, xid2: TransactionId :: {:add_to_pool "J", j} (1 <= j && j < n+1 && xid1 != xid2 && Set_Contains(locked_transactions[j], xid1) && Set_Contains(locked_transactions[j], xid2)) ==> !Conflict[xid1][xid2]);
+preserves {:layer 1} LockedNoConflicts(locked_transactions);
 
+function {:inline} CommittedSubsetLocked(locked_transactions: [ReplicaId](Set TransactionId), committed_transactions: Set TransactionId) : bool
+{
+    (forall {:pool "J"} j: int, xid0: TransactionId :: {:add_to_pool "J", j}
+        1 <= j && j < n+1 && Set_Contains(committed_transactions, xid0)
+        ==> Set_Contains(locked_transactions[j], xid0))
+}
 yield invariant {:layer 1} CommittedSubsetLocked();
-preserves {:layer 1} (forall {:pool "J"} j:int, xid0: TransactionId :: {:add_to_pool "J", j} 1 <= j && j < n+1 && Set_Contains(committed_transactions, xid0) ==> Set_Contains(locked_transactions[j], xid0));
+preserves {:layer 1} CommittedSubsetLocked(locked_transactions, committed_transactions);
 
 yield invariant {:layer 1} XidInLocked({:linear} xid: One TransactionId);
 preserves (forall {:pool "J"} j:int :: {:add_to_pool "J", j} 1 <= j && j < n+1 ==> Set_Contains(locked_transactions[j], xid->val));
